Use definitions for numbers like 32
This significantly speeds up some files, because the proof terms are
smaller.

After     | File Name               | Before    || Change
------------------------------------------------------------
12m59.96s | Total                   | 16m25.75s || -3m25.78s
------------------------------------------------------------
2m04.61s  | x86/instrrules          | 3m46.66s  || -1m42.04s
0m51.70s  | x86/globals             | 1m09.94s  || -0m18.23s
0m19.91s  | x86/cfuncspec           | 0m29.17s  || -0m09.26s
0m40.63s  | x86/call                | 0m48.88s  || -0m08.25s
0m18.43s  | x86/matcher             | 0m26.38s  || -0m07.94s
0m13.68s  | x86/inlinealloc         | 0m20.35s  || -0m06.67s
0m07.33s  | x86/xorswap             | 0m14.29s  || -0m06.95s
0m21.26s  | x86/listproof           | 0m26.50s  || -0m05.23s
0m15.51s  | x86/mulc                | 0m20.04s  || -0m04.52s
0m15.18s  | x86/macros              | 0m19.51s  || -0m04.33s
0m14.75s  | pointsto                | 0m19.55s  || -0m04.80s
0m11.65s  | x86/lifeimp             | 0m15.74s  || -0m04.08s
0m10.38s  | x86/win/pecoff          | 0m15.14s  || -0m04.75s
0m13.08s  | x86/wrapalloc           | 0m16.60s  || -0m03.52s
0m05.81s  | x86/fact                | 0m09.64s  || -0m03.83s
0m10.63s  | x86/screenproof         | 0m13.18s  || -0m02.54s
0m09.91s  | x86/specexamples        | 0m12.65s  || -0m02.74s
0m06.78s  | x86/program             | 0m08.82s  || -0m02.04s
0m11.60s  | x86/imp                 | 0m12.79s  || -0m01.18s
0m08.96s  | triple                  | 0m10.45s  || -0m01.48s
0m08.56s  | x86/cstringimp          | 0m10.06s  || -0m01.50s
0m14.47s  | x86/main                | 0m15.22s  || -0m00.75s
0m13.97s  | x86/programassemcorrect | 0m14.57s  || -0m00.59s
0m13.92s  | x86/instrcodec          | 0m14.12s  || -0m00.19s
0m13.09s  | spec                    | 0m12.28s  || +0m00.81s
0m11.57s  | bitsopsprops            | 0m11.76s  || -0m00.18s
0m11.37s  | bitstest                | 0m11.26s  || +0m00.10s
0m08.75s  | codec                   | 0m08.83s  || -0m00.08s
0m07.81s  | spectac                 | 0m07.55s  || +0m00.25s
0m07.74s  | regex                   | 0m07.47s  || +0m00.27s
0m07.00s  | x86/basic               | 0m07.10s  || -0m00.09s
0m06.75s  | x86/gcdex               | 0m06.78s  || -0m00.03s
0m06.66s  | septac                  | 0m06.71s  || -0m00.04s
0m06.47s  | safe                    | 0m06.31s  || +0m00.16s
0m06.27s  | x86/basicprog           | 0m06.16s  || +0m00.10s
0m05.71s  | x86/screenspec          | 0m05.84s  || -0m00.12s
0m05.69s  | x86/listspec            | 0m05.80s  || -0m00.10s
0m05.64s  | x86/examples            | 0m05.74s  || -0m00.10s
0m05.63s  | x86/testrun             | 0m05.93s  || -0m00.29s
0m05.58s  | x86/cfunc               | 0m05.69s  || -0m00.11s
0m05.56s  | x86/entry               | 0m05.51s  || +0m00.04s
0m05.55s  | SPred                   | 0m05.58s  || -0m00.03s
0m05.54s  | codecregex              | 0m05.56s  || -0m00.01s
0m05.53s  | x86/screenimp           | 0m05.72s  || -0m00.18s
0m05.51s  | x86/programeq           | 0m05.06s  || +0m00.45s
0m05.50s  | x86/listimp             | 0m05.72s  || -0m00.21s
0m05.27s  | x86/programassem        | 0m05.12s  || +0m00.14s
0m05.21s  | roundtrip               | 0m05.23s  || -0m00.02s
0m04.82s  | bitreader               | 0m05.01s  || -0m00.18s
0m04.79s  | x86/step                | 0m04.78s  || +0m00.00s
0m04.71s  | bitsprops               | 0m04.58s  || +0m00.12s
0m04.49s  | pmapprops               | 0m04.34s  || +0m00.15s
0m04.42s  | x86/eval                | 0m04.43s  || -0m00.00s
0m04.36s  | bitscodec               | 0m04.39s  || -0m00.02s
0m04.28s  | x86/encdechelp          | 0m04.38s  || -0m00.09s
0m04.25s  | writer                  | 0m04.37s  || -0m00.12s
0m04.23s  | reader                  | 0m04.10s  || +0m00.13s
0m04.23s  | cursor                  | 0m04.19s  || +0m00.04s
0m04.19s  | x86/procstatemonad      | 0m04.20s  || -0m00.00s
0m04.10s  | x86/procstate           | 0m04.07s  || +0m00.02s
0m04.06s  | x86/mem                 | 0m04.01s  || +0m00.04s
0m03.94s  | x86/reg                 | 0m03.91s  || +0m00.02s
0m03.81s  | bitsrep                 | 0m03.80s  || +0m00.01s
0m03.80s  | x86/ioaction            | 0m03.74s  || +0m00.05s
0m03.74s  | pmap                    | 0m03.66s  || +0m00.08s
0m03.74s  | x86/flags               | 0m03.66s  || +0m00.08s
0m03.70s  | bitsops                 | 0m03.66s  || +0m00.04s
0m03.65s  | x86/instrsyntax         | 0m03.61s  || +0m00.04s
0m03.63s  | enc                     | 0m03.57s  || +0m00.06s
0m03.61s  | x86/instr               | 0m03.57s  || +0m00.04s
0m03.60s  | x86/regstate            | 0m03.58s  || +0m00.02s
0m03.50s  | nathelp                 | 0m03.45s  || +0m00.04s
0m03.44s  | charge/iltac            | 0m03.30s  || +0m00.14s
0m02.62s  | charge/bilogic          | 0m02.67s  || -0m00.04s
0m02.56s  | charge/ilogic           | 0m02.52s  || +0m00.04s
0m02.37s  | charge/later            | 0m02.29s  || +0m00.08s
0m02.31s  | charge/sepalg           | 0m02.30s  || +0m00.01s
0m02.29s  | tuplehelp               | 0m02.21s  || +0m00.08s
0m02.27s  | ilogicss                | 0m02.26s  || +0m00.01s
0m02.17s  | sparsefun               | 0m02.18s  || -0m00.01s
0m02.12s  | monadinst               | 0m02.08s  || +0m00.04s
0m02.09s  | cast                    | 0m02.06s  || +0m00.02s
0m01.94s  | cstring                 | 0m01.89s  || +0m00.05s
0m01.91s  | monad                   | 0m01.87s  || +0m00.03s
0m01.87s  | emb                     | 0m01.84s  || +0m00.03s
0m01.77s  | x86/exn                 | 0m01.79s  || -0m00.02s
0m00.95s  | charge/CSetoid          | 0m00.94s  || +0m00.01s
0m00.93s  | pfun                    | 0m00.92s  || +0m00.01s
0m00.30s  | common_tactics          | 0m00.31s  || -0m00.01s
0m00.29s  | update                  | 0m00.30s  || -0m00.01s

src/bitreader.v
@@ -51,7 +51,9 @@ Qed.
    are the index of the current bit that we are reading, with 0 representing the *most*
    significant bit and 7 the least significant (this is the opposite to our usual
    ordering) *)
-Definition BitCursor := Cursor 35.
+Definition n35 := n32.+3.
+Arguments n35 : simpl never.
+Definition BitCursor := Cursor n35.
 
 (* Functional interpretation of bitReader on sequences. Returns the
    final position, the tail of the given sequence and the value
@@ -168,7 +170,7 @@ Inductive BBInv : BitCursor -> seq bool -> DWORDCursor -> seq bool -> seq BYTE -
   BBInv (p ## fromNat (n:=3) (7 - size accbits)) (accbit::accbits++toBin bytes)
   (next p) (accbit::accbits) bytes.
 
-Lemma BBInvProp1 (bytec: DWORD) (byte:BYTE) (bytes: seq BYTE) accbit accbits (p:BITS 35) :
+Lemma BBInvProp1 (bytec: DWORD) (byte:BYTE) (bytes: seq BYTE) accbit accbits (p:BITS n35) :
   fromByteCursor bytec = mkCursor p  ->
   rev byte = accbit :: accbits ->
   BBInv p (accbit :: accbits ++ toBin bytes) bytec [::] (byte :: bytes) ->
@@ -180,7 +182,7 @@ have: size (rev byte) = 8 by rewrite size_rev size_tuple. rewrite E2/=; congruen
 destruct accbits => //.
 injection E1 => <-. simpl.
 replace (zero 3) with (fromNat (n:=3) 0).
-have NC := @nextCat 32 3 bytec 0. rewrite NC => //.
+have NC := @nextCat n32 3 bytec 0. rewrite NC => //.
 simpl in SIZELO. injection SIZELO => SIZEACCBITS.
 replace (fromNat (n:=3) 1) with (fromNat (n:=3) (7 - size accbits)).
 apply BBInvCons. by rewrite SIZEACCBITS. by rewrite SIZEACCBITS.
@@ -250,8 +252,8 @@ Qed.
 (* Note that if bits is non-null then the byte cursor is already advanced to the next
    location *)
 Definition bitCursorAndBitsToByteCursor (c:BitCursor) (bits:seq bool) : DWORDCursor :=
-  if c is mkCursor p then if bits is nil then mkCursor (@high 32 3 p)
-                          else next (@high 32 3 p) else top _.
+  if c is mkCursor p then if bits is nil then mkCursor (@high n32 3 p)
+                          else next (@high n32 3 p) else top _.
 
 Corollary bitReaderToReader_correct t (br: BitReader t) :
   forall bytes resbits (cursor: DWORDCursor) (cursor':BitCursor) v,
